Interference.thy
@@ -2,48 +2,54 @@ theory Interference
   imports Semantics
 begin
 
-locale interference = semantics re fwd eval
-  for re :: "'a \<Rightarrow> 'a \<Rightarrow> bool" (infix "\<hookleftarrow>" 100)
-  and fwd :: "'a \<Rightarrow> 'a \<Rightarrow> 'a" ("_\<langle>_\<rangle>" [1000,0] 1000)
-  and eval :: "'a \<Rightarrow> 's rel"
+chapter \<open>Reordering Interference\<close>
+
+text \<open>
+Define the necessary side-conditions to ensure reordering cannot introduce interference.
+First defines properties to avoid interference for the early execution of an instruction,
+and then defines all possible early executions that may be observed for a program.
+\<close>
+
+locale interference = semantics
 
 context interference
 begin
 
 section \<open>Interference Definitions\<close>
 
-text \<open>Independence of two instructions \<beta> and \<alpha> under environment R, 
-      such that the early execution of \<alpha> is assumed to be possible and 
-      cannot invalidate sequential reasoning\<close>
-definition inter\<^sub>a
-  where "inter\<^sub>a R G \<beta> \<alpha> \<equiv> R\<^sup>* \<otimes> eval \<alpha>\<langle>\<beta>\<rangle> \<otimes> R\<^sup>* \<otimes> eval \<beta> \<subseteq> R\<^sup>* \<otimes> eval \<beta> \<otimes> R\<^sup>* \<otimes> eval \<alpha> \<and> guar \<alpha>\<langle>\<beta>\<rangle> G"
+text \<open>
+Independence of two instructions \<beta> and \<alpha> under environment R, 
+such that the early execution of \<alpha> is assumed to be possible and 
+cannot invalidate sequential reasoning.\<close>
+definition inter\<^sub>\<alpha> :: "'b rpred \<Rightarrow> 'b rpred \<Rightarrow> 'a \<Rightarrow> 'a \<Rightarrow> bool"
+  where "inter\<^sub>\<alpha> R G \<beta> \<alpha> \<equiv> R\<^sup>* O eval \<alpha>\<langle>\<beta>\<rangle> O R\<^sup>* O eval \<beta> \<subseteq> R\<^sup>* O eval \<beta> O R\<^sup>* O eval \<alpha> \<and> eval \<alpha>\<langle>\<beta>\<rangle> \<subseteq> G"
 
-text \<open>Independence of program c and instruction \<alpha> under environment R,
-      such that the early execution of \<alpha> is assumed to be possible and 
-      cannot invalidate sequential reasoning.
-      Define by recursively iterating over the program and capturing the forwarding throughout.\<close>
-fun inter\<^sub>c
+text \<open>
+Independence of program c and instruction \<alpha> under environment R,
+such that the early execution of \<alpha> is assumed to be possible and 
+cannot invalidate sequential reasoning.
+Define by recursively iterating over the program and capturing the forwarding throughout.\<close>
+fun inter\<^sub>c :: "'b rpred \<Rightarrow> 'b rpred \<Rightarrow> 'a com \<Rightarrow> 'a \<Rightarrow> bool"
   where
-    "inter\<^sub>c R G (Basic \<beta>) \<alpha> = inter\<^sub>a R G \<beta> \<alpha>" |
-    "inter\<^sub>c R G (c\<^sub>1 ; c\<^sub>2) \<alpha> = (inter\<^sub>c R G c\<^sub>1 \<alpha>\<llangle>c\<^sub>2\<rrangle> \<and> inter\<^sub>c R G c\<^sub>2 \<alpha>)" |
+    "inter\<^sub>c R G (Basic \<beta>) \<alpha> = inter\<^sub>\<alpha> R G \<beta> \<alpha>" |
+    "inter\<^sub>c R G (c\<^sub>1 ;; c\<^sub>2) \<alpha> = (inter\<^sub>c R G c\<^sub>1 \<alpha>\<llangle>c\<^sub>2\<rrangle> \<and> inter\<^sub>c R G c\<^sub>2 \<alpha>)" |
     "inter\<^sub>c R G (c\<^sub>1 \<sqinter> c\<^sub>2) \<alpha> = (inter\<^sub>c R G c\<^sub>1 \<alpha> \<and> inter\<^sub>c R G c\<^sub>2 \<alpha>)" |
     "inter\<^sub>c R G (c*) \<alpha> = inter\<^sub>c R G c \<alpha>" |
     "inter\<^sub>c R G _ \<alpha> = True"
 
-(* instrumented step c \<mapsto>[\<alpha>,r,\<alpha>'] c'
-   \<alpha> = fwd(\<alpha>'); 
-   r = "collects" all the steps that \<alpha>' got forwarded over to \<alpha> (in the middle parameter of \<mapsto>)
-       for each of these stmts in r non-interference with \<alpha> needs to be proved *)
-
-text \<open>Instrumented version of the semantics that collects the reordering effects\<close>
+text \<open>
+Instrumented version of the semantics that collects the reordering effects.
+Given c \<mapsto>[\<alpha>,r,\<alpha>'] c', this corresponds to c \<mapsto>\<alpha> c', such that
+r should be the program \<alpha>' has to reorder with in c to execute and 
+\<alpha> should be \<alpha>' forwarded across r.\<close>
 inductive_set execute_collect :: "('a com \<times> 'a \<times> 'a com \<times> 'a \<times> 'a com) set"
   and execute_collect_abv :: "'a com \<Rightarrow> 'a \<Rightarrow> 'a com \<Rightarrow> 'a \<Rightarrow> 'a com \<Rightarrow> bool"
   ("_ \<mapsto>[_,_,_] _" [71,0,0,0,71] 70)
   where
   "c \<mapsto>[\<alpha>,t,\<gamma>] c' \<equiv> (c, \<alpha>, t, \<gamma>, c') \<in> execute_collect" |
   act[intro]:  "Basic \<alpha> \<mapsto>[\<alpha>,Nil,\<alpha>] Nil" |
-  pre[intro]:  "c\<^sub>1 \<mapsto>[\<alpha>,c,\<alpha>'] c\<^sub>1' \<Longrightarrow> c\<^sub>1 ; c\<^sub>2 \<mapsto>[\<alpha>,c,\<alpha>'] c\<^sub>1' ; c\<^sub>2" |
-  pst[intro]:  "c\<^sub>1 \<mapsto>[\<alpha>,c,\<alpha>'] c\<^sub>1' \<Longrightarrow> \<gamma> < c\<^sub>2 <\<^sub>p \<alpha> \<Longrightarrow> c\<^sub>2 ; c\<^sub>1 \<mapsto>[\<gamma>,c\<^sub>2;c,\<alpha>'] c\<^sub>2 ; c\<^sub>1'"
+  pre[intro]:  "c\<^sub>1 \<mapsto>[\<alpha>,c,\<alpha>'] c\<^sub>1' \<Longrightarrow> c\<^sub>1 ;; c\<^sub>2 \<mapsto>[\<alpha>,c,\<alpha>'] c\<^sub>1' ;; c\<^sub>2" |
+  pst[intro]:  "c\<^sub>1 \<mapsto>[\<alpha>,c,\<alpha>'] c\<^sub>1' \<Longrightarrow> \<gamma> < c\<^sub>2 <\<^sub>c \<alpha> \<Longrightarrow> c\<^sub>2 ;; c\<^sub>1 \<mapsto>[\<gamma>,c\<^sub>2;;c,\<alpha>'] c\<^sub>2 ;; c\<^sub>1'"
 inductive_cases execute_collect[elim]: "c\<^sub>1 \<mapsto>[\<alpha>,c,\<alpha>'] c\<^sub>1'"
 
 text \<open>Compute possible reorderings of the program using the instrumented semantics\<close>
@@ -57,13 +63,15 @@ text \<open>Ensure all reorderings enforce the necessary interference property\<
 definition inter
   where "inter R G c \<equiv> \<forall>t. reorder_trace t c \<longrightarrow> (\<forall>(r,\<alpha>) \<in> set t. inter\<^sub>c R G r \<alpha>)"
 
-text \<open>Interference is preserved across a silent step\<close>
+section \<open>Interference Properties\<close>
+
+text \<open>Interference check is preserved across a silent step\<close>
 lemma inter_silentI [intro]:
   assumes "inter R G c" "c \<leadsto> c'"
   shows "inter R G c'"
   using assms by (auto simp: inter_def intro: reorder_trace.intros)
 
-text \<open>Interference is preserved across an execution step and prevents interference\<close>
+text \<open>Interference check is preserved across an execution step and prevents interference\<close>
 lemma indep_stepI [intro]:
   assumes "inter R G c" "c \<mapsto>[\<alpha>,r,\<alpha>'] c'"
   shows "inter R G c' \<and> inter\<^sub>c R G r \<alpha>'"
@@ -73,12 +81,12 @@ lemma indep_stepI [intro]:
 text \<open>Instrumented semantics collects valid reorderings\<close>
 lemma collect_reorder:
   assumes "c \<mapsto>[\<alpha>',r,\<alpha>] c'"
-  shows "\<alpha>' < r <\<^sub>p \<alpha>"
+  shows "\<alpha>' < r <\<^sub>c \<alpha>"
   using assms by (induct, auto)
 
 text \<open>Convert a normal execution step into an instrumented step\<close>
 lemma exec_collect:
-  assumes "c \<mapsto>\<^sub>\<alpha> c'" "local_only c"
+  assumes "c \<mapsto>\<^sub>\<alpha> c'" "local c"
   shows "\<exists>r \<alpha>'. c \<mapsto>[\<alpha>,r,\<alpha>'] c'"
   using assms by induct auto
 
