Local_Rules.thy
@@ -1,40 +1,20 @@
 theory Local_Rules
-  imports Semantics
+  imports Syntax
 begin
 
-chapter \<open>Thread Local Rules\<close>
+chapter \<open>Local Rules\<close>
 
-locale local_rules = semantics re fwd eval
-  for re :: "'a \<Rightarrow> 'a \<Rightarrow> bool" (infix "\<hookleftarrow>" 100)
-  and fwd :: "'a \<Rightarrow> 'a \<Rightarrow> 'a" ("_\<langle>_\<rangle>" [1000,0] 1000)
-  and eval :: "'a \<Rightarrow> 's rel"
+text \<open>Define the rely/guarantee rules for a local program.\<close>
 
-context local_rules
-begin
+section \<open>Helper Definitions\<close>
 
-section \<open>Rule Definitions\<close>
-
-text \<open>Stability of a state across an environment step\<close>
-definition stable
+text \<open>Stability of a predicate across an environment step\<close>
+definition stable :: "'a rel \<Rightarrow> 'a set \<Rightarrow> bool"
   where "stable R P \<equiv> \<forall>m m'. m \<in> P \<longrightarrow> (m,m') \<in> R \<longrightarrow> m' \<in> P"
 
-text \<open>Rule for an atomic operation with a context\<close>
-definition atomic_rule :: "'s rel \<Rightarrow> 's rel \<Rightarrow> 's set \<Rightarrow> 'a \<Rightarrow> 's set \<Rightarrow> bool" 
-  ("_,_ \<turnstile>\<^sub>A _ {_} _" [20, 20, 20, 20] 20)
-  where "R,G \<turnstile>\<^sub>A P {\<alpha>} Q \<equiv> P \<subseteq> wp \<alpha> Q \<and> guar \<alpha> G \<and> stable R P \<and> stable R Q"
-
-text \<open>Establish the rules of the logic, similar to standard Hoare-logic\<close>
-inductive lrules :: "'s rel \<Rightarrow> 's rel \<Rightarrow> 's set \<Rightarrow> 'a com \<Rightarrow> 's set \<Rightarrow> bool"
-  ("_,_ \<turnstile>\<^sub>t _ {_} _" [20,0,0,0,20] 20)
-where
-  nil[intro]:    "stable R P \<Longrightarrow> R,G \<turnstile>\<^sub>t P { Nil } P" |
-  seq[intro]:    "R,G \<turnstile>\<^sub>t P { c\<^sub>1 } Q \<Longrightarrow> R,G \<turnstile>\<^sub>t Q { c\<^sub>2 } M \<Longrightarrow> R,G \<turnstile>\<^sub>t P { c\<^sub>1 ; c\<^sub>2 } M" |
-  choice[intro]: "R,G \<turnstile>\<^sub>t P { c\<^sub>1 } Q \<Longrightarrow> R,G \<turnstile>\<^sub>t P { c\<^sub>2 } Q \<Longrightarrow> R,G \<turnstile>\<^sub>t P { c\<^sub>1 \<sqinter> c\<^sub>2 } Q" |
-  loop[intro]:   "stable R P \<Longrightarrow> R,G \<turnstile>\<^sub>t P { c } P \<Longrightarrow> R,G \<turnstile>\<^sub>t P { c* } P" |
-  basic[intro]:  "R,G \<turnstile>\<^sub>A P {\<alpha>} Q \<Longrightarrow> R,G \<turnstile>\<^sub>t P { Basic \<alpha> } Q" |
-  conseq[intro]: "R,G \<turnstile>\<^sub>t P { c } Q \<Longrightarrow> P' \<subseteq> P \<Longrightarrow> R' \<subseteq> R \<Longrightarrow> G \<subseteq> G' \<Longrightarrow> Q \<subseteq> Q' \<Longrightarrow> R',G' \<turnstile>\<^sub>t P' { c } Q'"
-
-section \<open>Helper Lemmas\<close>
+text \<open>Weakest precondition for an arbitrary state relation\<close>
+definition wp :: "'b rpred \<Rightarrow> 'b pred \<Rightarrow> 'b pred"
+  where "wp \<alpha> P \<equiv> {m. \<forall>m'. (m,m') \<in> \<alpha> \<longrightarrow> m' \<in> P}"
 
 lemma stable_conseqI [intro]:
   assumes "stable R' P" "R \<subseteq> R'" 
@@ -46,36 +26,56 @@ lemma stable_conjI [intro]:
   shows "stable (R \<inter> R') (P \<inter> P')"
   using assms by (auto simp: stable_def)
 
-lemma guar_conseqI [intro]:
-  assumes "G' \<subseteq> G" "guar \<alpha> G'"
-  shows "guar \<alpha> G"
-  using assms unfolding guar_def by auto
+lemma stable_transitive:
+  assumes "(m,m') \<in> R\<^sup>*" "m \<in> P" "stable R P"
+  shows "m' \<in> P"
+  using assms by (induct rule: rtrancl.induct) (auto simp: stable_def)
 
-lemma thread_only:
-  assumes "R,G \<turnstile>\<^sub>t P { c } Q"
-  shows "local_only c"
-  using assms by induct auto
+locale local_rules =
+  fixes eval :: "'a \<Rightarrow> 'b rel" 
 
-section \<open>Atomic Rules\<close>
+context local_rules
+begin
 
+section \<open>Atomic Rule\<close>
+
+text \<open>Weakest precondition for an instruction\<close>
+abbreviation wp\<^sub>\<alpha> :: "'a \<Rightarrow> 'b pred \<Rightarrow> 'b pred"
+  where "wp\<^sub>\<alpha> \<alpha> P \<equiv> wp (eval \<alpha>) P"
+
+text \<open>Specification Check, ensuring an instruction conforms to a relation\<close>
+abbreviation guar :: "'a \<Rightarrow> 'b rpred \<Rightarrow> bool"
+  where "guar \<alpha> G \<equiv> eval \<alpha> \<subseteq> G"
+
+text \<open>Rule for an atomic operation\<close>
+definition atomic_rule :: "'b rpred \<Rightarrow> 'b rpred \<Rightarrow> 'b pred \<Rightarrow> 'a \<Rightarrow> 'b pred \<Rightarrow> bool" 
+  ("_,_ \<turnstile>\<^sub>A _ {_} _" [40,0,0,0,40] 40)
+  where "R,G \<turnstile>\<^sub>A P {\<alpha>} Q \<equiv> P \<subseteq> wp\<^sub>\<alpha> \<alpha> Q \<and> guar \<alpha> G \<and> stable R P \<and> stable R Q"
+
+subsection \<open>Properties\<close>
+
+text \<open>Re-establish an atomic judgement over a stronger stable precondition\<close>
 lemma atomic_pre:
   assumes "R,G \<turnstile>\<^sub>A P {\<alpha>} Q" "P' \<subseteq> P" "stable R P'"
   shows "R,G \<turnstile>\<^sub>A P' {\<alpha>} Q"
   using assms unfolding atomic_rule_def
   by fast
 
+text \<open>Strengthen the rely and weaken the guarantee for an atomic judgement\<close>
 lemma atomic_conseqI [intro]:
   assumes "R,G \<turnstile>\<^sub>A P {\<alpha>} Q" "R' \<subseteq> R" "G \<subseteq> G'"
   shows "R',G' \<turnstile>\<^sub>A P {\<alpha>} Q"
-  using assms guar_conseqI unfolding atomic_rule_def
+  using assms unfolding atomic_rule_def
   by blast
 
+text \<open>Atomic judgements over the same instruction can be combined\<close>
 lemma actomic_conjI [intro]:
   assumes "R,G \<turnstile>\<^sub>A P\<^sub>1 {\<alpha>} Q\<^sub>1" "R,G  \<turnstile>\<^sub>A P\<^sub>2 {\<alpha>} Q\<^sub>2"
-  shows "R,G \<turnstile>\<^sub>A (P\<^sub>1 \<inter> P\<^sub>2) {\<alpha>} (Q\<^sub>1 \<inter> Q\<^sub>2)"
+  shows "R,G \<turnstile>\<^sub>A P\<^sub>1 \<inter> P\<^sub>2 {\<alpha>} Q\<^sub>1 \<inter> Q\<^sub>2"
   using assms unfolding atomic_rule_def  
   by (auto simp: wp_def stable_def)
 
+text \<open>Add an invariant across an atomic judgement\<close>
 lemma atomic_frameI [intro]:
   assumes "R,G \<turnstile>\<^sub>A P {\<alpha>} Q"
   assumes "stable R\<^sub>2 M" "G \<subseteq> R\<^sub>2"
@@ -84,21 +84,39 @@ lemma atomic_frameI [intro]:
 proof (safe, goal_cases)
   case (1 x)
   hence "{(m,m'). m \<in> P} \<inter> eval \<alpha> \<subseteq> R\<^sub>2" 
-    using assms(1,3) unfolding guar_def atomic_rule_def by fast
-  hence "x \<in> wp \<alpha> M" using assms(2) 1 unfolding stable_def wp_def by blast
-  moreover have "x \<in> wp \<alpha> Q" using 1 assms(1) by (auto simp: atomic_rule_def wp_def)
+    using assms(1,3) unfolding atomic_rule_def by fast
+  hence "x \<in> wp\<^sub>\<alpha> \<alpha> M" using assms(2) 1 unfolding stable_def wp_def by blast
+  moreover have "x \<in> wp\<^sub>\<alpha> \<alpha> Q" using 1 assms(1) by (auto simp: atomic_rule_def wp_def)
   ultimately show ?case by (auto simp: wp_def)
 qed (insert assms, auto simp: atomic_rule_def wp_def)
 
-section \<open>Elimination Rules\<close>
+section \<open>Local Rules\<close>
+
+text \<open>Rules of the logic over a thread, similar to standard Hoare-logic\<close>
+inductive lrules :: "'b rpred \<Rightarrow> 'b rpred \<Rightarrow> 'b pred \<Rightarrow> 'a com \<Rightarrow> 'b pred \<Rightarrow> bool" 
+  ("_,_ \<turnstile>\<^sub>l _ {_} _" [20,0,0,0,20] 20)
+where
+  nil[intro]:    "stable R P \<Longrightarrow> R,G \<turnstile>\<^sub>l P { Nil } P" |
+  seq[intro]:    "R,G \<turnstile>\<^sub>l P { c\<^sub>1 } Q \<Longrightarrow> R,G \<turnstile>\<^sub>l Q { c\<^sub>2 } M \<Longrightarrow> R,G \<turnstile>\<^sub>l P { c\<^sub>1 ;; c\<^sub>2 } M" |
+  choice[intro]: "R,G \<turnstile>\<^sub>l P { c\<^sub>1 } Q \<Longrightarrow> R,G \<turnstile>\<^sub>l P { c\<^sub>2 } Q \<Longrightarrow> R,G \<turnstile>\<^sub>l P { c\<^sub>1 \<sqinter> c\<^sub>2 } Q" |
+  loop[intro]:   "stable R P \<Longrightarrow> R,G \<turnstile>\<^sub>l P { c } P \<Longrightarrow> R,G \<turnstile>\<^sub>l P { c* } P" |
+  basic[intro]:  "R,G \<turnstile>\<^sub>A P {\<alpha>} Q \<Longrightarrow> R,G \<turnstile>\<^sub>l P { Basic \<alpha> } Q" |
+  conseq[intro]: "R,G \<turnstile>\<^sub>l P { c } Q \<Longrightarrow> P' \<subseteq> P \<Longrightarrow> R' \<subseteq> R \<Longrightarrow> G \<subseteq> G' \<Longrightarrow> Q \<subseteq> Q' \<Longrightarrow> R',G' \<turnstile>\<^sub>l P' { c } Q'"
+
+subsection \<open>Properties\<close>
+
+text \<open>
+Various elimination rules based on a judgement over a particular program structure.
+These mostly deal with complexities introduced by support conseq.
+\<close>
 
 lemma nilE [elim!]:
-  assumes "R,G \<turnstile>\<^sub>t P {Nil} Q"
+  assumes "R,G \<turnstile>\<^sub>l P {Nil} Q"
   obtains M where "stable R M" "P \<subseteq> M" "M \<subseteq> Q"
   using assms by (induct R G P "Nil :: 'a com" Q) blast+
 
 lemma basicE [elim!]:
-  assumes "R,G \<turnstile>\<^sub>t P {Basic \<beta>} Q"
+  assumes "R,G \<turnstile>\<^sub>l P {Basic \<beta>} Q"
   obtains P' Q' where "P \<subseteq> P'" "R,G \<turnstile>\<^sub>A P' {\<beta>} Q'" "Q' \<subseteq> Q"
   using assms 
 proof (induct R G P "Basic \<beta>" Q)
@@ -110,19 +128,19 @@ next
 qed
 
 lemma seqE [elim]:
-  assumes "R,G \<turnstile>\<^sub>t P {c\<^sub>1 ; c\<^sub>2} Q"
-  obtains M  where "R,G \<turnstile>\<^sub>t P {c\<^sub>1} M" "R,G \<turnstile>\<^sub>t M {c\<^sub>2} Q"
+  assumes "R,G \<turnstile>\<^sub>l P {c\<^sub>1 ;; c\<^sub>2} Q"
+  obtains M  where "R,G \<turnstile>\<^sub>l P {c\<^sub>1} M" "R,G \<turnstile>\<^sub>l M {c\<^sub>2} Q"
   using assms 
-  by (induct R G P "c\<^sub>1 ; c\<^sub>2" Q arbitrary: c\<^sub>1 c\<^sub>2) blast+
+  by (induct R G P "c\<^sub>1 ;; c\<^sub>2" Q arbitrary: c\<^sub>1 c\<^sub>2) blast+
 
 lemma choiceE [elim]:
-  assumes "R,G \<turnstile>\<^sub>t P {c\<^sub>1 \<sqinter> c\<^sub>2} Q"
-  obtains "R,G \<turnstile>\<^sub>t P {c\<^sub>1} Q" "R,G \<turnstile>\<^sub>t P {c\<^sub>2} Q"
+  assumes "R,G \<turnstile>\<^sub>l P {c\<^sub>1 \<sqinter> c\<^sub>2} Q"
+  obtains "R,G \<turnstile>\<^sub>l P {c\<^sub>1} Q" "R,G \<turnstile>\<^sub>l P {c\<^sub>2} Q"
   using assms by (induct R G P "c\<^sub>1 \<sqinter> c\<^sub>2" Q arbitrary: c\<^sub>1 c\<^sub>2) auto
 
 lemma loopE [elim]:
-  assumes "R,G \<turnstile>\<^sub>t P { c* } Q"
-  obtains I where "P \<subseteq> I" "R,G \<turnstile>\<^sub>t I { c } I" "I \<subseteq> Q" "stable R I"
+  assumes "R,G \<turnstile>\<^sub>l P { c* } Q"
+  obtains I where "P \<subseteq> I" "R,G \<turnstile>\<^sub>l I { c } I" "I \<subseteq> Q" "stable R I"
   using assms 
 proof (induct R G P "c*" Q arbitrary: c)
   case (loop R G P c)
@@ -132,19 +150,21 @@ next
   then show ?case using lrules.conseq stable_conseqI by (metis subset_eq)
 qed
 
-lemma parE [elim!]:
-  assumes "R,G \<turnstile>\<^sub>t P { c\<^sub>1 || c\<^sub>2 } Q"
-  obtains "False"
-  using assms 
-proof (induct R G P "c\<^sub>1 || c\<^sub>2" Q)
-  case (conseq R G P Q P' R' G' Q')
-  thus ?case by blast
-qed
+text \<open>No local judgement can be established over parallel composition\<close>
+lemma local_only:
+  assumes "R,G \<turnstile>\<^sub>l P { c } Q"
+  shows "local c"
+  using assms by induct auto
 
-text \<open>We can always weaken the precondition to a stable state\<close>
+lemma parE [elim!]:
+  assumes "R,G \<turnstile>\<^sub>l P { c\<^sub>1 || c\<^sub>2 } Q"
+  obtains "False"
+  using local_only assms by force
+
+text \<open>Weaken the precondition of a judgement to a stable state\<close>
 lemma stable_preE:
-  assumes "R,G \<turnstile>\<^sub>t P {c} Q"
-  obtains P' where "P \<subseteq> P'" "stable R P'" "R,G \<turnstile>\<^sub>t P' {c} Q"
+  assumes "R,G \<turnstile>\<^sub>l P {c} Q"
+  obtains P' where "P \<subseteq> P'" "stable R P'" "R,G \<turnstile>\<^sub>l P' {c} Q"
   using assms 
 proof (induct)
   case (basic R G P \<alpha> Q)
