Semantics.thy
@@ -4,8 +4,16 @@ begin
 
 chapter \<open>Small Step Semantics\<close>
 
+text \<open>
+Define the small step semantics for the While language, with weak memory model behaviours.
+Also introduces a notion of configuration, that couples programs and memory states,
+with transitions for the program and the environment.
+\<close>
+
+type_synonym ('a,'b) config = "'a com \<times> 'b"
+
 locale semantics = reordering +
-  fixes eval :: "'a \<Rightarrow> 's rel" 
+  fixes eval :: "'a \<Rightarrow> 'b rel" 
 
 context semantics
 begin
@@ -13,15 +21,15 @@ begin
 section \<open>Program Transition Definitions\<close>
 
 text \<open>Small step semantics for an instruction execution\<close>
-text \<open>To remove WMM from the theory, it suffices to remove the pst case below\<close>
+text \<open>To remove reordering from the theory, it suffices to remove the out-of-order (ooo) case below\<close>
 inductive_set execute :: "('a com \<times> 'a \<times> 'a com) set"
   and execute_abv :: "'a com \<Rightarrow> 'a \<Rightarrow> 'a com \<Rightarrow> bool"
-  ("_ \<mapsto>\<^sub>_ _" [71,0,71] 70)
+  ("_ \<mapsto>\<^sub>_ _" [71,73,71] 70)
   where
   "c \<mapsto>\<^sub>\<alpha> c' \<equiv> (c, \<alpha>, c') \<in> execute" |
   act[intro]:  "Basic \<alpha> \<mapsto>\<^sub>\<alpha> Nil" |
-  pre[intro]:  "c\<^sub>1 \<mapsto>\<^sub>\<alpha> c\<^sub>1' \<Longrightarrow> c\<^sub>1 ; c\<^sub>2 \<mapsto>\<^sub>\<alpha> c\<^sub>1' ; c\<^sub>2" |
-  pst[intro]:  "c\<^sub>1 \<mapsto>\<^sub>\<alpha> c\<^sub>1' \<Longrightarrow> \<gamma> < c\<^sub>2 <\<^sub>p \<alpha> \<Longrightarrow> c\<^sub>2 ; c\<^sub>1 \<mapsto>\<^sub>\<gamma> c\<^sub>2 ; c\<^sub>1'" |
+  seq[intro]:  "c\<^sub>1 \<mapsto>\<^sub>\<alpha> c\<^sub>1' \<Longrightarrow> c\<^sub>1 ;; c\<^sub>2 \<mapsto>\<^sub>\<alpha> c\<^sub>1' ;; c\<^sub>2" |
+  ooo[intro]:  "c\<^sub>1 \<mapsto>\<^sub>\<alpha> c\<^sub>1' \<Longrightarrow> \<gamma> < c\<^sub>2 <\<^sub>c \<alpha> \<Longrightarrow> c\<^sub>2 ;; c\<^sub>1 \<mapsto>\<^sub>\<gamma> c\<^sub>2 ;; c\<^sub>1'" |
   par1[intro]: "c\<^sub>1 \<mapsto>\<^sub>\<alpha> c\<^sub>1' \<Longrightarrow> c\<^sub>1 || c\<^sub>2 \<mapsto>\<^sub>\<alpha> c\<^sub>1' || c\<^sub>2" |
   par2[intro]: "c\<^sub>2 \<mapsto>\<^sub>\<alpha> c\<^sub>2' \<Longrightarrow> c\<^sub>1 || c\<^sub>2 \<mapsto>\<^sub>\<alpha> c\<^sub>1 || c\<^sub>2'"
 inductive_cases executeE[elim]: "c\<^sub>1 \<mapsto>\<^sub>\<alpha> c\<^sub>1'"
@@ -32,14 +40,14 @@ inductive_set silent :: "('a com \<times> 'a com) set"
   ("_ \<leadsto> _" [71,71] 70)
   where
   "c \<leadsto> c' \<equiv> (c, c') \<in> silent" |
-  seq1[intro]:  "c\<^sub>1 \<leadsto> c\<^sub>1' \<Longrightarrow> c\<^sub>1 ; c\<^sub>2 \<leadsto> c\<^sub>1' ; c\<^sub>2" |
-  seq2[intro]:  "c\<^sub>2 \<leadsto> c\<^sub>2' \<Longrightarrow> c\<^sub>1 ; c\<^sub>2 \<leadsto> c\<^sub>1 ; c\<^sub>2'" |
-  seqE1[intro]: "Nil ; c\<^sub>1 \<leadsto> c\<^sub>1" |
-  seqE2[intro]: "c\<^sub>1 ; Nil \<leadsto> c\<^sub>1" |
+  seq1[intro]:  "c\<^sub>1 \<leadsto> c\<^sub>1' \<Longrightarrow> c\<^sub>1 ;; c\<^sub>2 \<leadsto> c\<^sub>1' ;; c\<^sub>2" |
+  seq2[intro]:  "c\<^sub>2 \<leadsto> c\<^sub>2' \<Longrightarrow> c\<^sub>1 ;; c\<^sub>2 \<leadsto> c\<^sub>1 ;; c\<^sub>2'" |
+  seqE1[intro]: "Nil ;; c\<^sub>1 \<leadsto> c\<^sub>1" |
+  seqE2[intro]: "c\<^sub>1 ;; Nil \<leadsto> c\<^sub>1" |
   left[intro]:  "c\<^sub>1 \<sqinter> c\<^sub>2 \<leadsto> c\<^sub>1" |
   right[intro]: "c\<^sub>1 \<sqinter> c\<^sub>2 \<leadsto> c\<^sub>2" |
   loop1[intro]: "c* \<leadsto> Nil" |
-  loop2[intro]: "c* \<leadsto> c ; c*" |
+  loop2[intro]: "c* \<leadsto> c ;; c*" |
   par1[intro]:  "c\<^sub>1 \<leadsto> c\<^sub>1' \<Longrightarrow> c\<^sub>1 || c\<^sub>2 \<leadsto> c\<^sub>1' || c\<^sub>2" |
   par2[intro]:  "c\<^sub>2 \<leadsto> c\<^sub>2' \<Longrightarrow> c\<^sub>1 || c\<^sub>2 \<leadsto> c\<^sub>1 || c\<^sub>2'" |
   parE1[intro]: "Nil || c \<leadsto> c" |
@@ -47,38 +55,47 @@ inductive_set silent :: "('a com \<times> 'a com) set"
 inductive_cases silentE[elim]: "c\<^sub>1 \<leadsto> c\<^sub>1'"
 
 text \<open>An execution step implies the program has changed\<close>
-lemma step_neq:
+lemma execute_neq:
   assumes "c \<mapsto>\<^sub>\<alpha> c'"
   shows "c \<noteq> c'"
-  using assms
-  by (induct) auto
+  using assms by (induct) auto
 
 lemma [simp]:
   "c \<mapsto>\<^sub>\<alpha> c = False"
-  using step_neq by auto
+  using execute_neq by auto
+
+text \<open>A silent step will not introduce parallelism\<close>
+lemma local_silent:
+  "c \<leadsto> c' \<Longrightarrow> local c \<Longrightarrow> local c'"
+  by (induct rule: silent.induct) auto
+
+text \<open>An execution step will not introduce parallelism\<close>
+lemma local_execute:
+  "c \<mapsto>\<^sub>\<alpha> c' \<Longrightarrow> local c \<Longrightarrow> local c'"
+  by (induct rule: execute.induct) auto
 
 section \<open>Transition Definitions\<close>
 
 text \<open>These transitions are over configurations of (program,state)\<close>
 
 text \<open>Environment Transition\<close>
-abbreviation etran ("_ -e\<rightarrow> _" [81,81] 80)
-  where "etran s s' \<equiv> (fst s) = (fst s')"
+abbreviation env_tran :: "('a,'b) config \<Rightarrow> ('a,'b) config \<Rightarrow> bool" ("_ -e\<rightarrow> _" [81,81] 80)
+  where "s -e\<rightarrow> s' \<equiv> fst s = fst s'"
 
 text \<open>Program Execution Transition\<close>
-abbreviation ctran ("_ -\<alpha>\<rightarrow> _" [81,81] 80)
-  where "ctran s s' \<equiv> (\<exists>\<alpha>. ((fst s) \<mapsto>\<^sub>\<alpha> (fst s')) \<and> (snd s,snd s') \<in> eval \<alpha>)"
+abbreviation exec_tran :: "('a,'b) config \<Rightarrow> ('a,'b) config \<Rightarrow> bool" ("_ -\<alpha>\<rightarrow> _" [81,81] 80)
+  where "s -\<alpha>\<rightarrow> s' \<equiv> \<exists>\<alpha>. fst s \<mapsto>\<^sub>\<alpha> (fst s') \<and> (snd s,snd s') \<in> eval \<alpha>"
 
 text \<open>Program Silent Transition\<close>
-abbreviation stran ("_ -s\<rightarrow> _" [81,81] 80)
-  where "stran s s' \<equiv> (((fst s) \<leadsto> (fst s')) \<and> (snd s) = (snd s'))"
+abbreviation sil_tran :: "('a,'b) config \<Rightarrow> ('a,'b) config \<Rightarrow> bool" ("_ -s\<rightarrow> _" [81,81] 80)
+  where "s -s\<rightarrow> s' \<equiv> fst s \<leadsto> fst s' \<and> snd s = snd s'"
 
 text \<open>Program Transition\<close>
-abbreviation atran ("_ -c\<rightarrow> _" [81,81] 80)
-  where "atran s s' \<equiv> (s -\<alpha>\<rightarrow> s' \<or> s -s\<rightarrow> s')"
+abbreviation com_tran :: "('a,'b) config \<Rightarrow> ('a,'b) config \<Rightarrow> bool" ("_ -c\<rightarrow> _" [81,81] 80)
+  where "s -c\<rightarrow> s' \<equiv> s -\<alpha>\<rightarrow> s' \<or> s -s\<rightarrow> s'"
 
 text \<open>Collect of all possible transitions\<close>
-inductive_set transitions
+inductive_set transitions :: "('a,'b) config list set"
   where 
     one[intro]: "[s] \<in> transitions" |
     env[intro]: "s -e\<rightarrow> s' \<Longrightarrow> s'#t \<in> transitions \<Longrightarrow> s#s'#t \<in> transitions" |
@@ -86,37 +103,6 @@ inductive_set transitions
     sil[intro]: "s -s\<rightarrow> s' \<Longrightarrow> s'#t \<in> transitions \<Longrightarrow> s#s'#t \<in> transitions"
 inductive_cases transitionsE[elim]: "t \<in> transitions"
 
-text \<open>Ensure there is no parallelism within a program\<close>
-fun local_only
-  where 
-    "local_only (c\<^sub>1 || c\<^sub>2) = False" |
-    "local_only (c\<^sub>1 ; c\<^sub>2) = (local_only c\<^sub>1 \<and> local_only c\<^sub>2)" |    
-    "local_only (c\<^sub>1 \<sqinter> c\<^sub>2) = (local_only c\<^sub>1 \<and> local_only c\<^sub>2)" |  
-    "local_only (c*) = (local_only c)" |    
-    "local_only _ = True"
-
-lemma local_only_silent:
-  "c \<leadsto> c' \<Longrightarrow> local_only c \<Longrightarrow> local_only c'"
-  by (induct rule: silent.induct) auto
-
-section \<open>Predicate Manipulations\<close>
-
-text \<open>Weakest Precondition, based on evaluation of an instruction\<close>
-definition wp
-  where "wp a P \<equiv> {m. \<forall>m'. (m,m') \<in> eval a \<longrightarrow> m' \<in> P}"
-
-text \<open>Specification Check, ensuring an instruction conforms to a relation\<close>
-definition guar
-  where "guar \<alpha> G \<equiv> eval \<alpha> \<subseteq> G"
-
 end
-
-text \<open>Compose two state transitions\<close>
-definition comp (infixr "\<otimes>" 60)
-  where "comp a b \<equiv> {(m,m'). \<exists>m''. (m,m'') \<in> a \<and> (m'',m') \<in> b}"
-
-text \<open>Stabilisation of a predicate under an environment step\<close>
-definition st
-  where "st R P \<equiv> {m. \<forall>m'. (m,m') \<in> R\<^sup>* \<longrightarrow> m' \<in> P}"
 
 end
