Soundness.thy
@@ -9,127 +9,75 @@ locale soundness = global_rules
 context soundness
 begin
 
-section \<open>Soundness Definitions\<close>
+section \<open>Helper Definitions\<close>
 
-(* set of all traces that start at the beginning of c *)
-text \<open>Valid transitions starting from a particular program\<close>
-definition cp
-  where "cp c \<equiv> {t. t \<in> transitions \<and> fst (t ! 0) = c}"
+text \<open>Weakest precondition of the transitive closure of an arbitrary state relation\<close>
+abbreviation wp\<^sub>t :: "'b rpred \<Rightarrow> 'b pred \<Rightarrow> 'b pred"
+  where "wp\<^sub>t R P \<equiv> wp (R\<^sup>*) P"
 
-text \<open>Traces that satisfy a precondition\<close>
-definition pre
-  where "pre P \<equiv> {t. snd (t!0) \<in> P}"
+lemma stable_wp\<^sub>tI:
+  "stable R P \<Longrightarrow> P \<subseteq> wp\<^sub>t R P"
+  unfolding wp_def using stable_transitive by fast
 
-(* \<forall> i. (s\<^sub>i,s\<^sub>i') \<in> t\<^sub>e \<and> s\<^sub>i=(c\<^sub>i,m\<^sub>i) \<and> s\<^sub>i'=(c\<^sub>i',m\<^sub>i') \<rightarrow> (m\<^sub>i,m\<^sub>i') \<in> R  *)
-text \<open>Traces that satisfy a rely\<close>
-definition rely
-  where "rely R \<equiv> {t. (\<forall>i. Suc i < length t \<longrightarrow> t!i -e\<rightarrow> t!Suc i \<longrightarrow> (snd(t!i), snd(t!Suc i)) \<in> R)}"
-
-(* \<forall> i. (s\<^sub>i,s\<^sub>i') \<in> t\<^sub>p \<and> s\<^sub>i=(c\<^sub>i,m\<^sub>i) \<and> s\<^sub>i'=(c\<^sub>i',m\<^sub>i') \<rightarrow> (m\<^sub>i,m\<^sub>i') \<in> G  *)
-text \<open>Traces that satisfy a guarantee\<close>
-definition gur
-  where "gur G \<equiv> {t. (\<forall>i. Suc i < length t \<longrightarrow> t!i -c\<rightarrow> t!Suc i \<longrightarrow> (snd(t!i), snd(t!Suc i)) \<in> G\<^sup>=)}"
-
-text \<open>Traces that satisfy a postcondition\<close>
-definition post
-  where "post Q \<equiv> {t. fst (last t) = Nil \<longrightarrow> snd (last t) \<in> Q}"
-
-text \<open>Validity of the rely/guarantee judgements\<close>
-definition validity ("\<Turnstile> _ SAT [_, _, _, _]" [60,0,0,0,0] 45) 
-  where "\<Turnstile> c SAT [P, R, G, Q] \<equiv> cp c \<inter> pre P \<inter> rely R \<subseteq> gur G \<inter> post Q"
-
-text \<open>Strongest postcondition with N environment steps, 
+text \<open>Strongest postcondition across arbitrary environment steps, 
       used to compute some new intermediate states for reasoning\<close>
-definition sp
-  where "sp a R P \<equiv> {m. \<exists>m' m''. m' \<in> P \<and> (m',m'') \<in> eval a \<and> (m'',m) \<in> R\<^sup>* }"
+definition sp :: "'a \<Rightarrow> 'b rpred \<Rightarrow> 'b pred \<Rightarrow> 'b pred"
+  where "sp \<alpha> R P \<equiv> {m. \<exists>m' m''. m' \<in> P \<and> (m',m'') \<in> eval \<alpha> \<and> (m'',m) \<in> R\<^sup>* }"
 
-section \<open>Helper Lemmas\<close>
-
-lemma gur [simp]:
-  "(s # s' # t \<in> gur G) = (s' # t \<in> gur G \<and> (s -c\<rightarrow> s' \<longrightarrow> (snd s, snd s') \<in> G\<^sup>=))"
-  unfolding gur_def using length_Suc_conv less_Suc_eq_0_disj by auto
-
-lemma rely [simp]:
-  "(s # s' # t \<in> rely R) = (s' # t \<in> rely R \<and> (s -e\<rightarrow> s' \<longrightarrow> (snd s, snd s') \<in> R))"
-  unfolding rely_def using length_Suc_conv less_Suc_eq_0_disj by auto
-
-lemma pre [simp]:
-  "(s # t \<in> pre P) = (snd s \<in> P)"
-  by (auto simp: pre_def)
-
-lemma post [simp]:
-  "([x] \<in> post P) = (fst x = Nil \<longrightarrow> snd x \<in> P)"
-  "(s # s' # t \<in> post Q) = (s' # t \<in> post Q)"
-  by (auto simp: post_def)
-
-section \<open>Reordering Rules\<close> 
-
-subsection \<open>Some prelims for the reordering reasoning\<close>
-
-lemma stable_transitive:
-  assumes "(m,m') \<in> R\<^sup>*" "m \<in> P" "stable R P"
-  shows "m' \<in> P"
-  using assms by (induct rule: rtrancl.induct) (auto simp: stable_def)
-
-lemma stable_stI [intro]:
-  assumes "stable R P"
-  shows "P \<subseteq> st R P"
-  using assms stable_transitive by (auto simp: st_def)
-
+text \<open>Re-establish an atomic judgement with its strongest postcondition\<close>
 lemma atomic_strongest:
   assumes "R,G \<turnstile>\<^sub>A P {\<alpha>} Q"
-  shows "(R,G \<turnstile>\<^sub>A P {\<alpha>} (sp \<alpha> R P)) \<and> sp \<alpha> R P \<subseteq> Q"
+  shows "R,G \<turnstile>\<^sub>A P {\<alpha>} sp \<alpha> R P \<and> sp \<alpha> R P \<subseteq> Q"
 proof -
-  have "Q \<subseteq> st R Q" "P \<subseteq> wp \<alpha> Q" 
-    using assms stable_transitive unfolding atomic_rule_def st_def wp_def by fast+
-  hence "sp \<alpha> R P \<subseteq> Q" by (auto simp: sp_def wp_def st_def)
+  have "Q \<subseteq> {m. \<forall>m'. (m,m') \<in> R\<^sup>* \<longrightarrow> m' \<in> Q}" "P \<subseteq> wp\<^sub>\<alpha> \<alpha> Q" 
+    using assms stable_transitive unfolding atomic_rule_def wp_def by fast+
+  hence "sp \<alpha> R P \<subseteq> Q" by (auto simp: sp_def wp_def)
   moreover have "R,G \<turnstile>\<^sub>A P {\<alpha>} (sp \<alpha> R P)"
     using assms by (clarsimp simp add: atomic_rule_def wp_def stable_def sp_def) force
   ultimately show ?thesis by auto
 qed
 
-subsection \<open>Reordering with instructions and programs \<close>
+section \<open>Reordering Rules\<close> 
 
 text \<open>
   Reorder the judgements of two reorderable instructions given a suitable interference property.
   The precondition P and postcondition Q are preserved.
 \<close>
 lemma reorder_action:
-  assumes "R,G \<turnstile>\<^sub>A P {\<beta>} M" "R,G \<turnstile>\<^sub>A M {\<alpha>} Q" "\<beta> \<hookleftarrow> fwd \<alpha> \<beta>" "inter\<^sub>a R G \<beta> \<alpha>"
-  obtains M' where "R,G \<turnstile>\<^sub>A P {fwd \<alpha> \<beta>} M'" "R,G \<turnstile>\<^sub>A M' {\<beta>} Q"
+  assumes "R,G \<turnstile>\<^sub>A P {\<beta>} M" "R,G \<turnstile>\<^sub>A M {\<alpha>} Q" "\<beta> \<hookleftarrow> \<alpha>\<langle>\<beta>\<rangle>" "inter\<^sub>\<alpha> R G \<beta> \<alpha>"
+  obtains M' where "R,G \<turnstile>\<^sub>A P {\<alpha>\<langle>\<beta>\<rangle>} M'" "R,G \<turnstile>\<^sub>A M' {\<beta>} Q"
 proof -
   \<comment> \<open>Nominate the strongest-postcondition of \<alpha> from P as the state between \<alpha> and \<beta>\<close>
-  let ?\<alpha>="fwd \<alpha> \<beta>"
-  let ?M="sp ?\<alpha> R P"
+  let ?M="sp \<alpha>\<langle>\<beta>\<rangle> R P"
 
   \<comment> \<open>Extract order independence properties\<close>
-  have "R\<^sup>* \<otimes> eval ?\<alpha> \<otimes> R\<^sup>* \<otimes> eval \<beta> \<subseteq> R\<^sup>* \<otimes> eval \<beta> \<otimes> R\<^sup>* \<otimes> eval \<alpha>"
-    using assms(4) by (auto simp: inter\<^sub>a_def)
-  hence env: "\<forall>Q. st R (wp \<beta> (st R (wp \<alpha> Q))) \<subseteq> st R (wp ?\<alpha> (st R (wp \<beta> Q)))"
-    unfolding comp_def wp_def st_def by safe blast 
-  have g: "guar ?\<alpha> G" using assms(4) by (auto simp: inter\<^sub>a_def)
+  have "R\<^sup>* O eval \<alpha>\<langle>\<beta>\<rangle> O R\<^sup>* O eval \<beta> \<subseteq> R\<^sup>* O eval \<beta> O R\<^sup>* O eval \<alpha>"
+    using assms(4) by (auto simp: inter\<^sub>\<alpha>_def)
+  hence env: "\<forall>Q. wp\<^sub>t R (wp\<^sub>\<alpha> \<beta> (wp\<^sub>t R (wp\<^sub>\<alpha> \<alpha> Q))) \<subseteq> wp\<^sub>t R (wp\<^sub>\<alpha> \<alpha>\<langle>\<beta>\<rangle> (wp\<^sub>t R (wp\<^sub>\<alpha> \<beta> Q)))"
+    unfolding comp_def wp_def by safe blast 
+  have g: "eval \<alpha>\<langle>\<beta>\<rangle> \<subseteq> G" using assms(4) by (auto simp: inter\<^sub>\<alpha>_def)
 
   \<comment> \<open>Establish stability for P, Q and the new intermediate state, in addition to guarantees\<close>
-  have stablePQ: "stable R P" "stable R Q" "guar \<alpha> G" "guar \<beta> G"
+  have stablePQ: "stable R P" "stable R Q" "eval \<alpha> \<subseteq> G" "eval \<beta> \<subseteq> G"
     using assms(1,2) by (auto simp: atomic_rule_def)
   have stableM: "stable R ?M"  unfolding stable_def sp_def by force
 
   \<comment> \<open>Show transition from P to Q is independent of order\<close>
-  have p: "P \<subseteq> wp \<beta> M" "M \<subseteq> wp \<alpha> Q" "M \<subseteq> st R M" "P \<subseteq> st R P" "Q \<subseteq> st R Q"
-    using assms(1,2) stable_stI unfolding atomic_rule_def wp_def by auto
-  hence "P \<subseteq> st R (wp \<beta> (st R (wp \<alpha> Q)))" unfolding st_def wp_def by blast
-  hence exec: "P \<subseteq> st R (wp ?\<alpha> (st R (wp \<beta> Q)))" using env by blast
+  have p: "P \<subseteq> wp\<^sub>\<alpha> \<beta> M" "M \<subseteq> wp\<^sub>\<alpha> \<alpha> Q" "M \<subseteq> wp\<^sub>t R M" "P \<subseteq> wp\<^sub>t R P" "Q \<subseteq> wp\<^sub>t R Q"
+    using assms(1,2)  unfolding atomic_rule_def by (auto intro!: stable_wp\<^sub>tI)
+  hence "P \<subseteq> wp\<^sub>t R (wp\<^sub>\<alpha> \<beta> (wp\<^sub>t R (wp\<^sub>\<alpha> \<alpha> Q)))" unfolding wp_def by blast
+  hence exec: "P \<subseteq> wp\<^sub>t R (wp\<^sub>\<alpha> \<alpha>\<langle>\<beta>\<rangle> (wp\<^sub>t R (wp\<^sub>\<alpha> \<beta> Q)))" using env by blast
 
   \<comment> \<open>Establish the late judgement over \<beta>\<close>
   have "R,G \<turnstile>\<^sub>A ?M {\<beta>} Q" 
   proof (unfold atomic_rule_def, intro conjI Int_greatest)
-    show "?M \<subseteq> wp \<beta> Q" using exec unfolding st_def wp_def sp_def by blast
+    show "?M \<subseteq> wp (eval \<beta>) Q" using exec unfolding wp_def sp_def by blast
   qed (insert stablePQ stableM, simp)
 
   \<comment> \<open>Establish the early judgement over the new \<alpha>\<close>
-  moreover have "R,G \<turnstile>\<^sub>A P {?\<alpha>} ?M"
+  moreover have "R,G \<turnstile>\<^sub>A P {\<alpha>\<langle>\<beta>\<rangle>} ?M"
   proof (unfold atomic_rule_def, intro conjI Int_greatest)
-    show "P \<subseteq> wp ?\<alpha> ?M" unfolding wp_def wf_def sp_def by blast
+    show "P \<subseteq> wp\<^sub>\<alpha> \<alpha>\<langle>\<beta>\<rangle> ?M" unfolding wp_def wf_def sp_def by blast
   qed (insert stablePQ stableM g, simp)
 
   ultimately show ?thesis using that by blast
@@ -140,8 +88,8 @@ text \<open>
   interference property.
 \<close>
 lemma reorder_prog:
-  assumes "R,G \<turnstile>\<^sub>t P {c} M" "R,G \<turnstile>\<^sub>A M {\<alpha>} Q" "\<alpha>' < c <\<^sub>p \<alpha>" "inter\<^sub>c R G c \<alpha>"
-  obtains M' P' where "P \<subseteq> P'" "R,G \<turnstile>\<^sub>A P' {\<alpha>'} M'" "R,G \<turnstile>\<^sub>t M' {c} Q"
+  assumes "R,G \<turnstile>\<^sub>l P {c} M" "R,G \<turnstile>\<^sub>A M {\<alpha>} Q" "\<alpha>' < c <\<^sub>c \<alpha>" "inter\<^sub>c R G c \<alpha>"
+  obtains M' P' where "P \<subseteq> P'" "R,G \<turnstile>\<^sub>A P' {\<alpha>'} M'" "R,G \<turnstile>\<^sub>l M' {c} Q"
   using assms
 proof (induct c arbitrary: R G P M Q \<alpha>' \<alpha>)
   case Nil
@@ -155,17 +103,17 @@ next
     using atomic_pre[OF Basic(3)] \<beta>(2,3) Basic(3) by (auto simp: atomic_rule_def)
   obtain M' where m'': "R,G \<turnstile>\<^sub>A P' {\<alpha>\<langle>\<beta>\<rangle>} M'" "R,G \<turnstile>\<^sub>A M' {\<beta>} Q"
     using reorder_action[OF \<beta>(2) m'(1) \<alpha>(1)] Basic by auto
-  have "R,G \<turnstile>\<^sub>t M' {Basic \<beta>} Q" by (rule lrules.basic[OF m''(2)])
+  have "R,G \<turnstile>\<^sub>l M' {Basic \<beta>} Q" by (rule lrules.basic[OF m''(2)])
   then show ?case using Basic(1) \<beta>(1) m''(1) \<alpha>(2) by auto
 next
   case (Seq c\<^sub>1 c\<^sub>2)
-  obtain \<alpha>\<^sub>n where \<alpha>: "\<alpha>' < c\<^sub>1 <\<^sub>p \<alpha>\<^sub>n" "\<alpha>\<^sub>n < c\<^sub>2 <\<^sub>p \<alpha>" using Seq by auto
-  obtain M' where m: "R,G \<turnstile>\<^sub>t P {c\<^sub>1} M'" "R,G \<turnstile>\<^sub>t M' {c\<^sub>2} M" using Seq(4) by fast
+  obtain \<alpha>\<^sub>n where \<alpha>: "\<alpha>' < c\<^sub>1 <\<^sub>c \<alpha>\<^sub>n" "\<alpha>\<^sub>n < c\<^sub>2 <\<^sub>c \<alpha>" using Seq by auto
+  obtain M' where m: "R,G \<turnstile>\<^sub>l P {c\<^sub>1} M'" "R,G \<turnstile>\<^sub>l M' {c\<^sub>2} M" using Seq(4) by fast
   have i: "inter\<^sub>c R G c\<^sub>1 \<alpha>\<^sub>n" "inter\<^sub>c R G c\<^sub>2 \<alpha>" using Seq \<alpha> by auto
   show ?case
   proof (rule Seq(2)[OF _ m(2) Seq(5) \<alpha>(2) i(2)], goal_cases outer)
     case (outer P' N')
-    hence c1: "R,G \<turnstile>\<^sub>t P {c\<^sub>1} P'" using m(1) conseq by auto
+    hence c1: "R,G \<turnstile>\<^sub>l P {c\<^sub>1} P'" using m(1) conseq by auto
     show ?case 
     proof (rule Seq(1)[OF _ c1 outer(2) \<alpha>(1) i(1)], goal_cases inner)
       case (inner P'' M'')
@@ -174,8 +122,8 @@ next
   qed
 next
   case (Choice c\<^sub>1 c\<^sub>2)
-  hence \<alpha>: "\<alpha>' < c\<^sub>1 <\<^sub>p \<alpha>" "\<alpha>' < c\<^sub>2 <\<^sub>p \<alpha>" by auto
-  obtain m: "R,G \<turnstile>\<^sub>t P {c\<^sub>1} M" "R,G \<turnstile>\<^sub>t P {c\<^sub>2} M" using Choice(4) by blast
+  hence \<alpha>: "\<alpha>' < c\<^sub>1 <\<^sub>c \<alpha>" "\<alpha>' < c\<^sub>2 <\<^sub>c \<alpha>" by auto
+  obtain m: "R,G \<turnstile>\<^sub>l P {c\<^sub>1} M" "R,G \<turnstile>\<^sub>l P {c\<^sub>2} M" using Choice(4) by blast
   have i: "inter\<^sub>c R G c\<^sub>1 \<alpha>" "inter\<^sub>c R G c\<^sub>2 \<alpha>" using Choice by auto
   show ?case
   proof (rule Choice(2)[OF _ m(2) Choice(5) \<alpha>(2) i(2)], goal_cases outer)
@@ -183,20 +131,20 @@ next
     show ?case 
     proof (rule Choice(1)[OF _ m(1) Choice(5) \<alpha>(1) i (1)], goal_cases inner)
       case (inner P'' N'')
-      hence "R,G \<turnstile>\<^sub>t (N' \<inter> N'') {c\<^sub>1} Q"
+      hence "R,G \<turnstile>\<^sub>l (N' \<inter> N'') {c\<^sub>1} Q"
         using outer by (meson Int_lower2 subset_refl lrules.conseq)
-      moreover have "R,G \<turnstile>\<^sub>t (N' \<inter> N'') {c\<^sub>2} Q" 
+      moreover have "R,G \<turnstile>\<^sub>l (N' \<inter> N'') {c\<^sub>2} Q" 
         using inner outer by (meson Int_lower1 subset_refl lrules.conseq)
-      ultimately have "R,G \<turnstile>\<^sub>t (N' \<inter> N'') {c\<^sub>1 \<sqinter> c\<^sub>2} Q" by auto
+      ultimately have "R,G \<turnstile>\<^sub>l (N' \<inter> N'') {c\<^sub>1 \<sqinter> c\<^sub>2} Q" by auto
       moreover have "P \<subseteq> P' \<inter> P''" using outer inner by auto
       ultimately show ?case using actomic_conjI[OF outer(2) inner(2)] Choice(3) by blast 
     qed
   qed
 next
   case (Loop c)
-  then obtain I where i: "P \<subseteq> I" "R,G \<turnstile>\<^sub>t I {c} I" "stable R I" "I \<subseteq> M" by auto
+  then obtain I where i: "P \<subseteq> I" "R,G \<turnstile>\<^sub>l I {c} I" "stable R I" "I \<subseteq> M" by auto
   have [simp]: "\<alpha>' = \<alpha>" using Loop by auto
-  have \<alpha>: "\<alpha> < c <\<^sub>p \<alpha>" using Loop by auto
+  have \<alpha>: "\<alpha> < c <\<^sub>c \<alpha>" using Loop by auto
   have "R,G \<turnstile>\<^sub>A I {\<alpha>} Q" using Loop(4) i(3,4) by (meson atomic_pre)
   hence s: "R,G \<turnstile>\<^sub>A I {\<alpha>} (sp \<alpha> R I)" "sp \<alpha> R I \<subseteq> Q" using atomic_strongest by auto
   have d: "inter\<^sub>c R G c \<alpha>" using Loop by auto
@@ -206,9 +154,9 @@ next
     case (outer P' I')
     hence "R,G \<turnstile>\<^sub>A I {\<alpha>} I'" using i(3) by (meson atomic_pre)
     hence "sp \<alpha> R I \<subseteq> I'" using atomic_strongest by auto
-    hence "R,G \<turnstile>\<^sub>t (sp \<alpha> R I) {c} (sp \<alpha> R I)" using outer(3) lrules.conseq by simp
-    hence "R,G \<turnstile>\<^sub>t (sp \<alpha> R I) {c*} (sp \<alpha> R I)" using s(1) by (meson loop atomic_rule_def)
-    hence "R,G \<turnstile>\<^sub>t (sp \<alpha> R I) {c*} Q" using s(2) conseq by blast
+    hence "R,G \<turnstile>\<^sub>l (sp \<alpha> R I) {c} (sp \<alpha> R I)" using outer(3) lrules.conseq by simp
+    hence "R,G \<turnstile>\<^sub>l (sp \<alpha> R I) {c*} (sp \<alpha> R I)" using s(1) by (meson loop atomic_rule_def)
+    hence "R,G \<turnstile>\<^sub>l (sp \<alpha> R I) {c*} Q" using s(2) conseq by blast
     then show ?case using Loop(2)[OF i(1)] s(1) by simp
   qed
 qed auto
@@ -217,9 +165,9 @@ section \<open>Transition Rules\<close>
 
 text \<open>Local judgements are preserved across silent steps\<close>
 lemma rewriteI [intro]:
-  assumes "R,G \<turnstile>\<^sub>t P {c} Q"
+  assumes "R,G \<turnstile>\<^sub>l P {c} Q"
   assumes "c \<leadsto> c'"
-  shows "R,G \<turnstile>\<^sub>t P {c'} Q"
+  shows "R,G \<turnstile>\<^sub>l P {c'} Q"
   using assms
 proof (induct arbitrary: c' rule: lrules.induct)
   case (seq R G P c\<^sub>1 Q c\<^sub>2 M)
@@ -242,26 +190,26 @@ qed auto
 
 text \<open>Local judgements are preserved across reordered interference-free execution steps\<close>
 lemma stepI:
-  assumes "c \<mapsto>[\<alpha>,r,\<alpha>'] c'" "R,G \<turnstile>\<^sub>t P {c} Q"
+  assumes "c \<mapsto>[\<alpha>,r,\<alpha>'] c'" "R,G \<turnstile>\<^sub>l P {c} Q"
   assumes "inter\<^sub>c R G r \<alpha>'"
-  shows "\<exists>P' M. P \<subseteq> P' \<and> (R,G \<turnstile>\<^sub>A P' {\<alpha>} M) \<and> (R,G \<turnstile>\<^sub>t M {c'} Q)"
+  shows "\<exists>P' M. P \<subseteq> P' \<and> (R,G \<turnstile>\<^sub>A P' {\<alpha>} M) \<and> (R,G \<turnstile>\<^sub>l M {c'} Q)"
   using assms
 proof (induct arbitrary: P R G Q)
   case (act \<alpha>)
   then show ?case by (elim basicE) (meson atomic_rule_def nil lrules.conseq order_refl)
 next
   case (pre c\<^sub>1 \<alpha> c \<alpha>' c\<^sub>1' c\<^sub>2)
-  obtain M' where m: "R,G \<turnstile>\<^sub>t P {c\<^sub>1} M'" "R,G \<turnstile>\<^sub>t M' {c\<^sub>2} Q" using pre by fast
+  obtain M' where m: "R,G \<turnstile>\<^sub>l P {c\<^sub>1} M'" "R,G \<turnstile>\<^sub>l M' {c\<^sub>2} Q" using pre by fast
   then show ?case using pre(2)[OF m(1) pre(4)] m(2) by blast
 next
   case (pst c\<^sub>2 \<alpha> c \<alpha>' c\<^sub>2' \<gamma> c\<^sub>1)
-  obtain M' where m: "R,G \<turnstile>\<^sub>t P {c\<^sub>1} M'" "R,G \<turnstile>\<^sub>t M' {c\<^sub>2} Q" using pst by fast
-  have i: "inter\<^sub>c R G c\<^sub>1 (fwd_prog \<alpha>' c)" "inter\<^sub>c R G c \<alpha>'" using pst by auto
-  obtain P' M where m': "M' \<subseteq> P'" "R,G \<turnstile>\<^sub>A P' {\<alpha>} M" "R,G \<turnstile>\<^sub>t M {c\<^sub>2'} Q"
+  obtain M' where m: "R,G \<turnstile>\<^sub>l P {c\<^sub>1} M'" "R,G \<turnstile>\<^sub>l M' {c\<^sub>2} Q" using pst by fast
+  have i: "inter\<^sub>c R G c\<^sub>1 (\<alpha>'\<llangle>c\<rrangle>)" "inter\<^sub>c R G c \<alpha>'" using pst by auto
+  obtain P' M where m': "M' \<subseteq> P'" "R,G \<turnstile>\<^sub>A P' {\<alpha>} M" "R,G \<turnstile>\<^sub>l M {c\<^sub>2'} Q"
     using pst(2)[OF m(2) i(2)] by blast
-  hence m'': "R,G \<turnstile>\<^sub>t P {c\<^sub>1} P'" using m(1) by blast
-  have "fwd_prog \<alpha>' c = \<alpha>" using pst(1) collect_reorder by auto
-  then show ?case using reorder_prog[OF m'' m'(2) pst(3)] i(1) m'(3) by (metis seq)
+  hence m'': "R,G \<turnstile>\<^sub>l P {c\<^sub>1} P'" using m(1) by blast
+  have "\<alpha>'\<llangle>c\<rrangle> = \<alpha>" using pst(1) collect_reorder by auto
+  then show ?case using reorder_prog[OF m'' m'(2) pst(3)] i(1) m'(3) by (metis lrules.seq)
 qed 
 
 text \<open>Global judgements are preserved across execution steps - reordering or not \<close>
@@ -303,24 +251,69 @@ next
   thus ?case using rules.frame atomic_frameI frame(3,4) by blast
 next
   case (thread R G P c Q)
-  hence "local_only c" using thread_only by auto
+  hence "local c" using local_only by auto
   then obtain r \<alpha>'' where c: "c \<mapsto>[\<alpha>,r,\<alpha>''] c'" using thread exec_collect by blast
   then show ?case 
     using stepI[OF c thread(1)] thread(2) indep_stepI[OF thread(2) c] by auto 
 qed
 
-section \<open>Sound Transition Theorem\<close>
+section \<open>Soundness\<close>
+
+text \<open>Set of all config traces that start with a program c\<close>
+definition cp :: "'a com \<Rightarrow> ('a,'b) config list set"
+  where "cp c \<equiv> {t. t \<in> transitions \<and> fst (t ! 0) = c}"
+
+text \<open>Set of all config traces that satisfy a precondition in their first state\<close>
+definition pre :: "'b pred \<Rightarrow> ('a,'b) config list set"
+  where "pre P \<equiv> {t. snd (t!0) \<in> P}"
+
+text \<open>Set of all config traces where environment steps satisfy a rely\<close>
+definition rely :: "'b rpred \<Rightarrow> ('a,'b) config list set"
+  where "rely R \<equiv> {t. (\<forall>i. Suc i < length t \<longrightarrow> t!i -e\<rightarrow> t!Suc i \<longrightarrow> (snd(t!i), snd(t!Suc i)) \<in> R)}"
+
+text \<open>Set of all config traces where program steps satisfy a guarantee\<close>
+definition gurn :: "'b rpred \<Rightarrow> ('a,'b) config list set"
+  where "gurn G \<equiv> {t. (\<forall>i. Suc i < length t \<longrightarrow> t!i -c\<rightarrow> t!Suc i \<longrightarrow> (snd(t!i), snd(t!Suc i)) \<in> G\<^sup>=)}"
+
+text \<open>Set of all config traces that satisfy a postcondition in their final state\<close>
+definition post :: "'b pred \<Rightarrow> ('a,'b) config list set"
+  where "post Q \<equiv> {t. fst (last t) = Nil \<longrightarrow> snd (last t) \<in> Q}"
+
+text \<open>Validity of the rely/guarantee judgements\<close>
+definition validity ("\<Turnstile> _ SAT [_, _, _, _]" [60,0,0,0,0] 45) 
+  where "\<Turnstile> c SAT [P, R, G, Q] \<equiv> cp c \<inter> pre P \<inter> rely R \<subseteq> gurn G \<inter> post Q"
+
+subsection \<open>Properties\<close>
+
+lemma gurn [simp]:
+  "(s # s' # t \<in> gurn G) = (s' # t \<in> gurn G \<and> (s -c\<rightarrow> s' \<longrightarrow> (snd s, snd s') \<in> G\<^sup>=))"
+  unfolding gurn_def using length_Suc_conv less_Suc_eq_0_disj by auto
+
+lemma rely [simp]:
+  "(s # s' # t \<in> rely R) = (s' # t \<in> rely R \<and> (s -e\<rightarrow> s' \<longrightarrow> (snd s, snd s') \<in> R))"
+  unfolding rely_def using length_Suc_conv less_Suc_eq_0_disj by auto
+
+lemma pre [simp]:
+  "(s # t \<in> pre P) = (snd s \<in> P)"
+  by (auto simp: pre_def)
+
+lemma post [simp]:
+  "([x] \<in> post P) = (fst x = Nil \<longrightarrow> snd x \<in> P)"
+  "(s # s' # t \<in> post Q) = (s' # t \<in> post Q)"
+  by (auto simp: post_def)
+
+subsection \<open>Soundness Proof\<close>
 
 text \<open>All transitions that start with a program with a logic judgement and satisfy
       the precondition and environment rely should conform to the guarantee and
       establish the postcondition if they terminate\<close>
 lemma sound_transitions:
   assumes "t \<in> transitions" "fst (t ! 0) = c" "R,G \<turnstile> P {c} Q" "t \<in> pre P \<inter> rely R"
-  shows "t \<in> gur G \<inter> post Q"
+  shows "t \<in> gurn G \<inter> post Q"
   using assms
 proof (induct arbitrary: c P rule: transitions.induct)
   case (one s)
-  thus ?case using gur_def by force
+  thus ?case using gurn_def by force
 next
   case (env s s' t)
   then obtain P' where "P \<subseteq> P'" "stable R P'" "R,G \<turnstile> P' {c} Q" by (metis g_stable_preE) 
@@ -330,13 +323,12 @@ next
   then obtain \<alpha> where \<alpha>: "c \<mapsto>\<^sub>\<alpha> (fst s')" "(snd s,snd s') \<in> eval \<alpha>" by auto
   then obtain P' M where "P \<subseteq> P'" "R,G \<turnstile>\<^sub>A P' {\<alpha>} M" "R,G \<turnstile> M {fst s'} Q"
     using g_stepI[OF prg(5) \<alpha>(1)] by metis
-  thus ?case using prg \<alpha> unfolding atomic_rule_def wp_def guar_def by fastforce
+  thus ?case using prg \<alpha> unfolding atomic_rule_def wp_def by fastforce
 next
   case (sil s s' t)
   thus ?case by auto
 qed
 
-text \<open>Soundness Theorem\<close>
 theorem sound:
   assumes "R,G \<turnstile> P { c } Q"
   shows "\<Turnstile> c SAT [P, R, G, Q]"
