Syntax.thy
@@ -2,16 +2,27 @@ theory Syntax
   imports Main
 begin
 
-chapter \<open>Syntax\<close>
+chapter \<open>While Language Syntax\<close>
 
-text \<open>Basic While Language syntax, with parallel composition\<close>
+type_synonym 'b pred = "'b set"
+type_synonym 'b rpred = "'b rel"
 
+text \<open>A While language with non-deterministic choice, iteration and parallel composition.\<close>
 datatype 'a com =
   Nil
   | Basic "'a"
-  | Seq "'a com" "'a com" (infixr ";" 80)
+  | Seq "'a com" "'a com" (infixr ";;" 80)
   | Choice "'a com" "'a com" (infixr "\<sqinter>" 150)
   | Loop "'a com" ("_*" [100] 150)
   | Parallel "'a com" "'a com"  (infixr "||" 150)
+
+text \<open>Ensure there is no parallelism within a program\<close>
+fun local :: "'a com \<Rightarrow> bool"
+  where 
+    "local (c\<^sub>1 || c\<^sub>2) = False" |
+    "local (c\<^sub>1 ;; c\<^sub>2) = (local c\<^sub>1 \<and> local c\<^sub>2)" |    
+    "local (c\<^sub>1 \<sqinter> c\<^sub>2) = (local c\<^sub>1 \<and> local c\<^sub>2)" |  
+    "local (c*) = (local c)" |    
+    "local _ = True"
 
 end
